Move some lemmas
Things about dest_closure and evaluate (and not the logical relation)
should be in closProps. This probably doesn't get all of them.

compiler/backend/semantics/closPropsScript.sml
@@ -1,6 +1,18 @@
 open preamble closLangTheory closSemTheory
 
 val _ = new_theory"closProps"
+ 
+val revdroprev = Q.store_thm("revdroprev",
+  `∀l n.
+     n ≤ LENGTH l ⇒ (REVERSE (DROP n (REVERSE l)) = TAKE (LENGTH l - n) l)`,
+  ho_match_mp_tac listTheory.SNOC_INDUCT >> simp[] >> rpt strip_tac >>
+  qcase_tac `n ≤ SUC (LENGTH l)` >>
+  `n = 0 ∨ ∃m. n = SUC m` by (Cases_on `n` >> simp[]) >> simp[]
+  >- simp[TAKE_APPEND2] >>
+  simp[TAKE_APPEND1] >>
+  `LENGTH l + 1 - SUC m = LENGTH l - m`
+     suffices_by (disch_then SUBST_ALL_TAC >> simp[]) >>
+  simp[]);
 
 val dec_clock_code = Q.store_thm("dec_clock_code",
   `(dec_clock x y).code = y.code`,
@@ -430,5 +442,429 @@ val lookup_vars_MEM = prove(
   \\ Cases_on `lookup_vars ys env2` \\ fs []
   \\ Cases_on `n` \\ fs [] \\ SRW_TAC [] [] \\ fs []) |> SPEC_ALL
   |> curry save_thm "lookup_vars_MEM";
+
+val bool_case_eq = Q.prove(
+  `COND b t f = v ⇔ b /\ v = t ∨ ¬b ∧ v = f`,
+  rw[] >> metis_tac[]);
+
+val clock_lemmas = Q.store_thm ("clock_lemmas",
+`!s. (s with clock := s.clock) = s`,
+ rw [state_component_equality]);
+
+val evaluate_app_rw = Q.store_thm ("evaluate_app_rw",
+`(!args loc_opt f s.
+  args ≠ [] ⇒
+  evaluate_app loc_opt f args s =
+    case dest_closure loc_opt f args of
+       | NONE => (Rerr(Rabort Rtype_error),s)
+       | SOME (Partial_app v) =>
+           if s.clock < LENGTH args then
+             (Rerr(Rabort Rtimeout_error),s with clock := 0)
+           else (Rval [v], dec_clock (LENGTH args) s)
+       | SOME (Full_app exp env rest_args) =>
+           if s.clock < (LENGTH args - LENGTH rest_args) then
+             (Rerr(Rabort Rtimeout_error),s with clock := 0)
+           else
+             case evaluate ([exp],env,dec_clock (LENGTH args - LENGTH rest_args) s) of
+                | (Rval [v], s1) =>
+                    evaluate_app loc_opt v rest_args s1
+                | res => res)`,
+ Cases_on `args` >>
+ fs [evaluate_def]);
+
+val op_thms = { nchotomy = op_nchotomy, case_def = op_case_def}
+val list_thms = { nchotomy = list_nchotomy, case_def = list_case_def}
+val option_thms = { nchotomy = option_nchotomy, case_def = option_case_def}
+val v_thms = { nchotomy = v_nchotomy, case_def = v_case_def}
+val ref_thms = { nchotomy = ref_nchotomy, case_def = ref_case_def}
+val result_thms = { nchotomy = TypeBase.nchotomy_of ``:('a,'b)result``,
+                    case_def = TypeBase.case_def_of ``:('a,'b)result`` }
+val appkind_thms = { nchotomy = TypeBase.nchotomy_of ``:app_kind``,
+                     case_def = TypeBase.case_def_of ``:app_kind`` }
+val eqs = LIST_CONJ (map prove_case_eq_thm [op_thms, list_thms, option_thms, v_thms, ref_thms, result_thms, appkind_thms])
+
+val _ = save_thm ("eqs", eqs);
+
+val pair_case_eq = Q.prove (
+`pair_CASE x f = v ⇔ ?x1 x2. x = (x1,x2) ∧ f x1 x2 = v`,
+ Cases_on `x` >>
+ rw []);
+
+val bool_case_eq = Q.prove(
+  `COND b t f = v ⇔ b /\ v = t ∨ ¬b ∧ v = f`,
+  rw[] >> metis_tac[]);
+
+val pair_lam_lem = Q.prove (
+`!f v z. (let (x,y) = z in f x y) = v ⇔ ∃x1 x2. z = (x1,x2) ∧ (f x1 x2 = v)`,
+ rw []);
+
+val do_app_cases_val = save_thm ("do_app_cases_val",
+``do_app op vs s = Rval (v,s')`` |>
+  (SIMP_CONV (srw_ss()++COND_elim_ss) [PULL_EXISTS, do_app_def, eqs, pair_case_eq, pair_lam_lem] THENC
+   SIMP_CONV (srw_ss()++COND_elim_ss) [LET_THM, eqs] THENC
+   ALL_CONV));
+
+val do_app_cases_err = save_thm ("do_app_cases_err",
+``do_app op vs s = Rerr (Rraise v)`` |>
+  (SIMP_CONV (srw_ss()++COND_elim_ss) [PULL_EXISTS, do_app_def, eqs, pair_case_eq, pair_lam_lem] THENC
+   SIMP_CONV (srw_ss()++COND_elim_ss) [LET_THM, eqs] THENC
+   ALL_CONV));
+
+val do_app_cases_timeout = save_thm ("do_app_cases_timeout",
+``do_app op vs s = Rerr (Rabort Rtimeout_error)`` |>
+  (SIMP_CONV (srw_ss()++COND_elim_ss) [PULL_EXISTS, do_app_def, eqs, pair_case_eq, pair_lam_lem] THENC
+   SIMP_CONV (srw_ss()++COND_elim_ss) [LET_THM, eqs] THENC
+   ALL_CONV));
+
+val dest_closure_none_loc = Q.store_thm ("dest_closure_none_loc",
+`!l cl vs v e env rest.
+  (dest_closure l cl vs = SOME (Partial_app v) ⇒ l = NONE) ∧
+  (dest_closure l cl vs = SOME (Full_app e env rest) ∧ rest ≠ [] ⇒ l = NONE)`,
+ rpt gen_tac >>
+ simp [dest_closure_def] >>
+ Cases_on `cl` >>
+ simp [] >>
+ rw [] >>
+ Cases_on `l` >>
+ fs [check_loc_def] >>
+ rw [] >>
+ rfs [DROP_NIL] >>
+ Cases_on `EL n l1` >>
+ fs [] >>
+ rw [] >>
+ rfs [DROP_NIL]);
+
+val is_closure_def = Define `
+(is_closure (Closure _ _ _ _ _) ⇔ T) ∧
+(is_closure (Recclosure _ _ _ _ _) ⇔ T) ∧
+(is_closure _ ⇔ F)`;
+
+val clo_to_loc_def = Define `
+(clo_to_loc (Closure l _ _ _ _) = l) ∧
+(clo_to_loc (Recclosure l _ _ _ i) = OPTION_MAP ((+) i) l)`;
+
+val clo_to_env_def = Define `
+(clo_to_env (Closure _ _ env _ _) = env) ∧
+(clo_to_env (Recclosure loc _ env fns _) =
+  GENLIST (Recclosure loc [] env fns) (LENGTH fns) ++ env)`;
+
+val clo_to_partial_args_def = Define `
+(clo_to_partial_args (Closure _ args _ _ _) = args) ∧
+(clo_to_partial_args (Recclosure _ args _ _ _) = args)`;
+
+val clo_add_partial_args_def = Define `
+(clo_add_partial_args args (Closure x1 args' x2 x3 x4) =
+  Closure x1 (args ++ args') x2 x3 x4) ∧
+(clo_add_partial_args args (Recclosure x1 args' x2 x3 x4) =
+  Recclosure x1 (args ++ args') x2 x3 x4)`;
+
+val clo_to_num_params_def = Define `
+(clo_to_num_params (Closure _ _ _ n _) = n) ∧
+(clo_to_num_params (Recclosure _ _ _ fns i) = FST (EL i fns))`;
+
+val rec_clo_ok_def = Define `
+(rec_clo_ok (Recclosure _ _ _ fns i) ⇔ i < LENGTH fns) ∧
+(rec_clo_ok (Closure _ _ _ _ _) ⇔ T)`;
+
+val dest_closure_full_length = Q.store_thm ("dest_closure_full_length",
+`!l v vs e args rest.
+  dest_closure l v vs = SOME (Full_app e args rest)
+  ⇒
+  LENGTH (clo_to_partial_args v) < clo_to_num_params v ∧
+  LENGTH vs + LENGTH (clo_to_partial_args v) = clo_to_num_params v + LENGTH rest ∧
+  LENGTH args = clo_to_num_params v + LENGTH (clo_to_env v)`,
+ rpt gen_tac >>
+ simp [dest_closure_def] >>
+ BasicProvers.EVERY_CASE_TAC >>
+ fs [is_closure_def, clo_to_partial_args_def, clo_to_num_params_def, clo_to_env_def]
+ >- (`n - LENGTH l' ≤ LENGTH vs` by decide_tac >>
+     rw [] >>
+     simp [LENGTH_TAKE]) >>
+ Cases_on `EL n l1` >>
+ fs [] >>
+ rw [] >>
+ simp []);
+
+val evaluate_app_clock_less = Q.store_thm ("evaluate_app_clock_less",
+`!loc_opt f args s1 vs s2.
+  args ≠ [] ∧
+  evaluate_app loc_opt f args s1 = (Rval vs, s2)
+  ⇒
+  s2.clock < s1.clock`,
+ rw [] >>
+ rfs [evaluate_app_rw] >>
+ BasicProvers.EVERY_CASE_TAC >>
+ fs [] >>
+ rw [] >>
+ TRY decide_tac >>
+ imp_res_tac evaluate_SING >>
+ fs [] >>
+ imp_res_tac evaluate_clock >>
+ fs [dec_clock_def] >>
+ imp_res_tac dest_closure_full_length >>
+ TRY decide_tac >>
+ Cases_on `args` >>
+ fs [] >>
+ decide_tac);
+
+val clo_add_partial_args_nil = Q.store_thm ("clo_add_partial_args_nil[simp]",
+`!x. is_closure x ⇒ clo_add_partial_args [] x = x`,
+ Cases_on `x` >>
+ rw [is_closure_def, clo_add_partial_args_def]);
+
+val clo_can_apply_def = Define `
+clo_can_apply loc cl num_args ⇔
+  LENGTH (clo_to_partial_args cl) < clo_to_num_params cl ∧
+  rec_clo_ok cl ∧
+  (loc ≠ NONE ⇒
+   loc = clo_to_loc cl ∧
+   num_args = clo_to_num_params cl ∧
+   clo_to_partial_args cl = [])`;
+
+val check_closures_def = Define `
+check_closures cl cl' ⇔
+  !loc num_args.
+    clo_can_apply loc cl num_args ⇒ clo_can_apply loc cl' num_args`;
+
+val dest_closure_partial_is_closure = Q.store_thm(
+  "dest_closure_partial_is_closure",
+  `dest_closure l v vs = SOME (Partial_app v') ⇒
+   is_closure v'`,
+  dsimp[dest_closure_def, eqs, bool_case_eq, is_closure_def, UNCURRY]);
+
+val is_closure_add_partial_args_nil = Q.store_thm(
+  "is_closure_add_partial_args_nil",
+  `is_closure v ⇒ (clo_add_partial_args [] v = v)`,
+  Cases_on `v` >> simp[]);
+
+val evaluate_app_clock0 = Q.store_thm(
+  "evaluate_app_clock0",
+  `s0.clock = 0 ∧ args ≠ [] ⇒
+   evaluate_app lopt r args s0 ≠ (Rval vs, s)`,
+  strip_tac >> `∃a1 args0. args = a1::args0` by (Cases_on `args` >> fs[]) >>
+  simp[evaluate_def] >>
+  Cases_on `dest_closure lopt r (a1::args0)` >> simp[] >>
+  qcase_tac `dest_closure lopt r (a1::args0) = SOME c` >>
+  Cases_on `c` >> simp[] >>
+  qcase_tac `dest_closure lopt r (a1::args0) = SOME (Full_app b env rest)` >>
+  rw[] >>
+  `SUC (LENGTH args0) ≤ LENGTH rest` by simp[] >>
+  imp_res_tac dest_closure_full_length >> lfs[])
+
+val evaluate_app_clock_drop = Q.store_thm(
+  "evaluate_app_clock_drop",
+  `∀args f lopt s0 s vs.
+     evaluate_app lopt f args s0 = (Rval vs, s) ⇒
+     s.clock + LENGTH args ≤ s0.clock`,
+  gen_tac >> completeInduct_on `LENGTH args` >>
+  full_simp_tac (srw_ss() ++ DNF_ss) [] >> qx_gen_tac `args` >>
+  `args = [] ∨ ∃a1 as. args = a1::as` by (Cases_on `args` >> simp[]) >>
+  dsimp[evaluate_def, eqs, bool_case_eq, pair_case_eq, dec_clock_def] >>
+  rpt strip_tac >> imp_res_tac evaluate_SING >> fs[] >> rw[] >>
+  qcase_tac `evaluate_app lopt r1 args' s1` >>
+  Cases_on `args' = []`
+  >- (fs[evaluate_def] >> rw[] >> imp_res_tac evaluate_clock >> fs[] >> simp[])
+  >- (`SUC (LENGTH as) ≤ LENGTH args' + s0.clock` by simp[] >>
+      `LENGTH args' < SUC (LENGTH as)`
+        by (imp_res_tac dest_closure_full_length >> lfs[]) >>
+      `s.clock + LENGTH args' ≤ s1.clock` by metis_tac[] >>
+      imp_res_tac evaluate_clock  >> fs[] >> simp[]))
+
+val dest_closure_is_closure = Q.store_thm(
+  "dest_closure_is_closure",
+  `dest_closure lopt f vs = SOME r ⇒ is_closure f`,
+  Cases_on `f` >> simp[is_closure_def, dest_closure_def]);
+
+val stage_partial_app = Q.store_thm(
+  "stage_partial_app",
+  `is_closure c ∧
+   dest_closure NONE v (rest ++ used) =
+     SOME (Partial_app (clo_add_partial_args rest c)) ⇒
+   dest_closure NONE c rest =
+     SOME (Partial_app (clo_add_partial_args rest c))`,
+  Cases_on `v` >> simp[dest_closure_def, eqs, bool_case_eq, UNCURRY] >>
+  Cases_on `c` >>
+  simp[clo_add_partial_args_def, is_closure_def, check_loc_def]);
+
+val dest_closure_full_addargs = Q.store_thm(
+  "dest_closure_full_addargs",
+  `dest_closure NONE c vs = SOME (Full_app b env r) ∧
+   LENGTH more + LENGTH vs ≤ max_app ⇒
+   dest_closure NONE c (more ++ vs) = SOME (Full_app b env (more ++ r))`,
+  Cases_on `c` >> csimp[dest_closure_def, bool_case_eq, revdroprev, UNCURRY] >>
+  simp[DROP_APPEND1, revdroprev, TAKE_APPEND1, TAKE_APPEND2] >>
+  simp[check_loc_def]);
+ 
+val evaluate_append = Q.store_thm  ("evaluate_append",
+`!es1 es2 env s.
+  evaluate (es1 ++ es2, env, s) =
+    case evaluate (es1, env, s) of
+    | (Rval vs1, s') =>
+        (case evaluate (es2, env, s') of
+         | (Rval vs2, s'') => (Rval (vs1++vs2), s'')
+         | x => x)
+    | x => x`,
+ Induct_on `es1` >>
+ rw [evaluate_def]
+ >- (
+   every_case_tac >>
+   rw []) >>
+ ONCE_REWRITE_TAC [evaluate_CONS] >>
+ every_case_tac >>
+ rw []);
+
+val evaluate_length_imp = Q.store_thm ("evaluate_length_imp",
+`evaluate (es,env,s1) = (Rval vs, s2) ⇒ LENGTH es = LENGTH vs`,
+ rw [] >>
+ Q.ISPECL_THEN [`es`, `env`, `s1`] mp_tac (hd (CONJUNCTS evaluate_LENGTH)) >>
+ rw []);
+
+val evaluate_app_length_imp = Q.store_thm ("evaluate_app_length_imp",
+`evaluate_app l f args s = (Rval vs, s2) ⇒ LENGTH vs = 1`,
+ rw [] >>
+ Q.ISPECL_THEN [`l`, `f`, `args`, `s`] mp_tac (hd (tl (CONJUNCTS evaluate_LENGTH))) >>
+ rw []);
+
+val dest_closure_none_append = Q.store_thm ("dest_closure_none_append",
+`!l f args1 args2. 
+  dest_closure NONE f args2 = NONE ⇒
+  dest_closure NONE f (args1 ++ args2) = NONE`,
+ rw [dest_closure_def] >>
+ Cases_on `f` >>
+ fs [check_loc_def] >>
+ rw [] >>
+ fs [LET_THM] >>
+ every_case_tac >>
+ fs [] >>
+ simp []);
+
+val dest_closure_none_append2 = Q.store_thm ("dest_closure_none_append2",
+`!l f args1 args2. 
+  LENGTH args1 + LENGTH args2 ≤ max_app ∧
+  dest_closure NONE f (args1 ++ args2) = NONE ⇒
+  dest_closure NONE f args2 = NONE`,
+ rw [dest_closure_def] >>
+ Cases_on `f` >>
+ fs [check_loc_def] >>
+ rw [] >>
+ fs [LET_THM] >>
+ every_case_tac >>
+ fs [] >>
+ simp []);
+
+val dest_closure_rest_length = Q.store_thm ("dest_closure_rest_length",
+`dest_closure NONE f args = SOME (Full_app e l rest) ⇒ LENGTH rest < LENGTH args`,
+ simp [dest_closure_def] >>
+ Cases_on `f` >>
+ simp [check_loc_def]
+ >- (rw [] >> simp []) >>
+ Cases_on `EL n l1`
+ >- (rw [] >> simp []));
+
+val dest_closure_partial_twice = Q.store_thm ("dest_closure_partial_twice",
+`∀f args1 args2 cl res.
+  LENGTH args1 + LENGTH args2 ≤ max_app ∧
+  dest_closure NONE f (args1 ++ args2) = res ∧
+  dest_closure NONE f args2 = SOME (Partial_app cl)
+  ⇒
+  dest_closure NONE cl args1 = res`,
+ simp [dest_closure_def] >>
+ Cases_on `f` >>
+ simp [check_loc_def]
+ >- (
+   Cases_on `cl` >>
+   simp [] >>
+   TRY (rw [] >> NO_TAC) >>
+   rw [] >>
+   simp [TAKE_APPEND, DROP_APPEND] >>
+   full_simp_tac (srw_ss()++ARITH_ss) [NOT_LESS, NOT_LESS_EQUAL]
+   >- (
+     Q.ISPECL_THEN [`REVERSE args2`, `n - LENGTH l`] mp_tac TAKE_LENGTH_TOO_LONG >>
+     rw [] >>
+     full_simp_tac (srw_ss()++ARITH_ss) [])
+   >- (
+     Q.ISPECL_THEN [`REVERSE args2`, `n - LENGTH l`] mp_tac DROP_LENGTH_TOO_LONG >>
+     rw [] >>
+     full_simp_tac (srw_ss()++ARITH_ss) []) >>
+   CCONTR_TAC >>
+   fs [] >>
+   rw [] >>
+   full_simp_tac (srw_ss()++ARITH_ss) []) >>
+ Cases_on `EL n l1` >>
+ fs [] >>
+ Cases_on `cl` >>
+ simp [] >>
+ TRY (rw [] >> NO_TAC) >>
+ rw [] >>
+ simp [TAKE_APPEND, DROP_APPEND] >>
+ full_simp_tac (srw_ss()++ARITH_ss) [NOT_LESS, NOT_LESS_EQUAL] >>
+ rw []
+ >- (
+   Q.ISPECL_THEN [`REVERSE args2`, `q - LENGTH l`] mp_tac TAKE_LENGTH_TOO_LONG >>
+   rw [] >>
+   full_simp_tac (srw_ss()++ARITH_ss) [])
+ >- (
+   Q.ISPECL_THEN [`REVERSE args2`, `q - LENGTH l`] mp_tac DROP_LENGTH_TOO_LONG >>
+   rw [] >>
+   full_simp_tac (srw_ss()++ARITH_ss) []));
+
+val evaluate_app_append = Q.store_thm ("evaluate_app_append",
+`!args2 f args1 s.
+  LENGTH (args1 ++ args2) ≤ max_app ⇒
+  evaluate_app NONE f (args1 ++ args2) s =
+    case evaluate_app NONE f args2 s of
+    | (Rval vs1, s1) => evaluate_app NONE (HD vs1) args1 s1
+    | err => err`,
+ gen_tac >>
+ completeInduct_on `LENGTH args2` >>
+ rw [] >>
+ Cases_on `args1++args2 = []`
+ >- fs [evaluate_def, APPEND_eq_NIL] >>
+ Cases_on `args2 = []`
+ >- fs [evaluate_def, APPEND_eq_NIL] >>
+ rw [evaluate_app_rw] >>
+ `dest_closure NONE f args2 = NONE ∨ ?x. dest_closure NONE f args2 = SOME x` by metis_tac [option_nchotomy] >>
+ fs []
+ >- (
+   imp_res_tac dest_closure_none_append >>
+   rw []) >>
+ Cases_on `x` >>
+ fs []
+ >- ( (* args2 partial app *)
+   `dest_closure NONE f (args1++args2) = NONE ∨
+    ?x. dest_closure NONE f (args1++args2) = SOME x` by metis_tac [option_nchotomy] >>
+   simp []
+   >- (imp_res_tac dest_closure_none_append2 >> fs []) >>
+   imp_res_tac dest_closure_partial_twice >>
+   rw [] >>
+   simp [] >>
+   Cases_on `x` >>
+   simp [] >>
+   full_simp_tac (srw_ss()++ARITH_ss) [NOT_LESS] >>
+   imp_res_tac dest_closure_rest_length >>
+   full_simp_tac (srw_ss()++ARITH_ss) [NOT_LESS] >>
+   Cases_on `args1 = []` >>
+   full_simp_tac (srw_ss()++ARITH_ss) [] >>
+   fs [evaluate_app_rw, dec_clock_def] >>
+   simp [evaluate_def] >>
+   rw [] >>
+   full_simp_tac (srw_ss()++ARITH_ss) [NOT_LESS])
+ >- ( (* args2 full app *)
+   imp_res_tac dest_closure_full_addargs >>
+   simp [] >>
+   rw [] >>
+   every_case_tac >>
+   imp_res_tac evaluate_SING >>
+   fs [] >>
+   rw [] >>
+   first_x_assum (qspec_then `LENGTH l0` mp_tac) >>
+   rw [] >>
+   `LENGTH l0 < LENGTH args2` by metis_tac [dest_closure_rest_length] >>
+   fs [] >>
+   first_x_assum (qspec_then `l0` mp_tac) >>
+   rw [] >>
+   pop_assum (qspecl_then [`h`, `args1`, `r`] mp_tac) >>
+   simp []));
+
 
 val _ = export_theory();
